src/StepM.v
@@ -3,7 +3,8 @@ Require Import Common FMap Syntax Semantics.
 
 Open Scope fmap.
 
-Inductive step_m (sys: System): MState -> MLabel -> MState -> Prop :=
+Inductive step_m {oifc} (sys: System oifc):
+  MState oifc -> MLabel -> MState oifc -> Prop :=
 | SmSlt: forall st, step_m sys st (RlblEmpty _) st
 | SmIns: forall pst nst oss orqs msgs eins,
     eins <> nil ->
@@ -24,9 +25,7 @@ Inductive step_m (sys: System): MState -> MLabel -> MState -> Prop :=
              bst_msgs := deqMsgs (idsOf eouts) msgs
           |} ->
     step_m sys pst (RlblOuts eouts) nst
-| SmInt: forall oidx obj rule
-                pst nst oss orqs msgs os porq pos norq ins iouts
-                (Hifc: ost_ifc os = obj_ifc obj),
+| SmInt: forall oidx obj rule pst nst oss orqs msgs os porq pos norq ins iouts,
     In obj (sys_objs sys) ->
     In rule (obj_rules obj) ->
     oidx = obj_idx obj ->
@@ -39,15 +38,15 @@ Inductive step_m (sys: System): MState -> MLabel -> MState -> Prop :=
     idsOf ins = rule_msgs_from rule porq ->
     map msg_id (valsOf ins) = rule_msg_ids rule ->
 
-    rule_precond rule (match Hifc with eq_refl => ost_st os end) porq ins ->
-    rule_trs rule (match Hifc with eq_refl => ost_st os end) porq ins =
+    rule_precond rule os porq ins ->
+    rule_trs rule os porq ins =
     (pos, norq, iouts) ->
     ValidMsgsOut sys iouts ->
 
     DisjList (idsOf ins) (idsOf iouts) ->
 
     pst = {| bst_oss := oss; bst_orqs := orqs; bst_msgs := msgs |} ->
-    nst = {| bst_oss := oss +[ oidx <- {| ost_st := pos |} ];
+    nst = {| bst_oss := oss +[ oidx <- pos ];
              bst_orqs := orqs +[ oidx <- norq ];
              bst_msgs := enqMsgs iouts (deqMsgs (idsOf ins) msgs)
           |} ->
